\documentclass[12pt,prb,aps,notitlepage]{revtex4-1}
\usepackage {amsmath}
\usepackage{amssymb}
\pdfoutput = 1 
\usepackage {graphicx}
\newcommand{\bomega}{\mbox{\boldmath$\omega$}}
\allowdisplaybreaks

\begin{document}

\title{Resistive Wall Mode}
\author{R.~Fitzpatrick\,\footnote{rfitzp@utexas.edu}}
\affiliation{Institute for Fusion Studies,  Department of Physics,  University of Texas at Austin,  Austin TX 78712, USA}\begin{abstract}
\end{abstract}
\maketitle

\section{Vacuum Solution}

\subsection{Normalization}
Let all lengths be normalized to the major radius of the magnetic axis, $R_0$. Let all
magnetic field-strengths be normalized to the toroidal magnetic field-strength at the magnetic axis, $B_0$.

\subsection{Toroidal Coordinates}
Let $\mu$, $\eta$, $\phi$ be toroidal coordinates such that
\begin{align}
R &= \frac{\sinh\mu}{\cosh\mu-\cos\eta},\\[0.5ex]
Z&=\frac{\sin\eta}{\cosh\mu-\cos\eta},
\end{align}
where $R$, $\phi$, $Z$ are cylindrical coordinates. 
The scale-factors of the toroidal coordinate system are
\begin{align}
h_\mu&=h_\eta= \frac{1}{\cosh\mu-\cos\eta}=h,\\[0.5ex]
h_\phi &= \frac{\sinh\mu}{\cosh\mu-\cos\eta} = h\,\sinh\mu.
\end{align}

\subsection{Perturbed Magnetic Field}
The perturbed magnetic field in the vacuum region is written
\begin{equation}
{\bf b} = {\rm i}\,\nabla \left[V(\mu,\eta)\,{\rm e}^{-{\rm i}\,n\,\phi}\right],
\end{equation}
where
\begin{align}
\nabla^2 V &= (z-\cos\eta)^3\left\{\frac{\partial}{\partial z}\!\left[\frac{z^2-1}{z-\cos\eta}\,\frac{\partial V}{\partial z}\right]\right.\nonumber\\[0.5ex]
&\left.\phantom{=}+\frac{\partial}{\partial \eta}\!\left[\frac{1}{z-\cos\eta}\,\frac{\partial V}{\partial\eta}\right]
-\frac{n^2\,V}{(z^2-1)\,(z-\cos\eta)}\right\}=0.
\end{align}
Here, $z=\cosh\mu$. 

Let
\begin{align}
f_z &= z^2-1,\\[0.5ex]
f_\eta &= (z-\cos\eta)^{1/2}.
\end{align}
It follows that
\begin{align}
\frac{df_z}{dz} &= 2\,z,\\[0.5ex]
\frac{\partial f_\eta}{\partial z}&= \frac{1}{2\,f_\eta},\\[0.5ex]
\frac{\partial f_\eta}{\partial\eta} &= \frac{\sin\eta}{2\,f_\eta}.
\end{align}

Let
\begin{equation}
V(z,\eta)= \sum_m f_\eta\,U_m(z)\,{\rm e}^{-{\rm i}\,m\,\eta}.
\end{equation}
Then, taking the sum and eikonal as read, and letting $'=d/dz$, we get 
\begin{align}
\frac{\partial V}{\partial z} &=\frac{U_m}{2\,f_\eta} + f_\eta\,U_m',\\[0.5ex]
\frac{\partial}{\partial z}\!\left(\frac{f_z}{f_\eta^{\,2}}\,\frac{\partial V}{\partial z}\right)&=
\frac{\partial}{\partial z}\!\left(\frac{f_z\,U_m}{2\,f_\eta^{\,3}}+ \frac{f_z\,U_m'}{f_\eta}\right)
= \frac{z\,U_m}{f_\eta^{\,3}} -\frac{3\,f_z\,U_m}{4\,f_\eta^{\,5}}+\frac{f_z\,U_m'}{2\,f_\eta^{\,3}}
+\frac{2\,z\,U_m'}{f_\eta}- \frac{f_z\,U_m'}{2\,f_\eta^{\,3}}
+\frac{f_z\,U_m''}{f_\eta}\nonumber\\[0.5ex]
&=\frac{z\,U_m}{f_\eta^{\,3}} -\frac{3\,(z^2-1)\,U_m}{4\,f_\eta^{\,5}}
+\frac{2\,z\,U_m'}{f_\eta}
+\frac{(z^2-1)\,U_m''}{f_\eta},\\[0.5ex]
\frac{\partial V}{\partial \eta} &=\frac{\sin\eta\,U_m}{2\,f_\eta} -{\rm i}\,m f_\eta\,U_m,\\[0.5ex]
\frac{\partial}{\partial \eta}\!\left(\frac{1}{f_\eta^{\,2}}\,\frac{\partial V}{\partial \eta}\right)&=
\frac{\partial}{\partial \eta}\!\left(\frac{\sin\eta\,U_m}{2\,f_\eta^{\,3}}-\frac{{\rm i}\,m\,U_m}{f_\eta}\right)=
\frac{\cos\eta\,U_m}{2\,f_\eta^{\,3}}- \frac{3\,\sin^2\eta\,U_m}{4\,f_\eta^{\,5}}-\frac{{\rm i}\,m\,\sin\eta\,U_m}{2\,f_\eta^{\,3}}\nonumber\\[0.5ex]
&\phantom{=} + \frac{{\rm i}\,m\,\sin\eta\,U_m}{2\,f_\eta^{\,3}} - \frac{m^2\,U_m}{f_\eta}\nonumber\\[0.5ex]
&=\frac{\cos\eta\,U_m}{2\,f_\eta^{\,3}}- \frac{3\,\sin^2\eta\,U_m}{4\,f_\eta^{\,5}} - \frac{m^2\,U_m}{f_\eta},\\[0.5ex]
-\frac{n^2\,V}{f_z\,f_\eta^{\,2}}&= -\frac{n^2\,U_m}{(z^2-1)\,f_\eta}.
\end{align}
Thus,
\begin{align}
0&=\frac{\partial}{\partial z}\!\left(\frac{f_z}{f_\eta^{\,2}}\,\frac{\partial V}{\partial z}\right)+ \frac{\partial}{\partial \eta}\!\left(\frac{1}{f_\eta^{\,2}}\,\frac{\partial V}{\partial \eta}\right)
-\frac{n^2\,V}{f_z\,f_\eta^{\,2}}\nonumber\\[0.5ex]&
= \frac{z\,U_m}{f_\eta^{\,3}} -\frac{3\,(z^2-1)\,U_m}{4\,f_\eta^{\,5}}
+\frac{2\,z\,U_m'}{f_\eta}
+\frac{(z^2-1)\,U_m''}{f_\eta}\nonumber\\[0.5ex]
&\phantom{=}+\frac{\cos\eta\,U_m}{2\,f_\eta^{\,3}}- \frac{3\,\sin^2\eta\,U_m}{4\,f_\eta^{\,5}} - \frac{m^2\,U_m}{f_\eta} -\frac{n^2\,U_m}{(z^2-1)\,f_\eta}\nonumber\\[0.5ex]
&=\frac{1}{f_\eta}\left[(z^2-1)\,U_m'' + 2\,z\,U_m' + \left(\frac{1}{4}-m^2\right)U_m - \frac{n^2\,U_m}{z^2-1}\right].
\end{align}
The most general solution of the previous equation is
\begin{equation}
U_m(z) = p_m\,P_{m-1/2}^{\,n}(z)+q_m\,Q_{m-1/2}^{\,n}(z),
\end{equation}
where $p_m$ and $q_m$ are arbitrary complex coefficients. 
Note that
\begin{align}
P_{-m-1/2}^{\,n}(z) &= P_{m-1/2}^{\,n}(z),\\[0.5ex]
Q_{-m-1/2}^{\,n}(z) &= Q_{m-1/2}^{\,n}(z),
\end{align}
so 
\begin{equation}
U_m(z) = p_m\,P_{|m|-1/2}^{\,n}(z)+q_m\,Q_{|m|-1/2}^{\,n}(z),
\end{equation}

Let
\begin{align}
p_m&= \bar{p}_m\,\hat{p}_m,\\[0.5ex]
q_m &= \bar{q}_m\,\hat{q}_m,
\end{align}
where
\begin{align}
\bar{p}_{m\neq 0}&= \cos(|m|\,\pi)\,\frac{\sqrt{\pi}\,\Gamma(|m|+1/2-n)\,\epsilon^{\,|m|}}{2^{|m|-1/2}\,|m|!},\\[0.5ex]
\bar{q}_{m\neq 0} &= \cos(n\,\pi)\,\cos(|m|\,\pi)\,\frac{2^{|m|+1/2}\,(|m|-1)!\,\epsilon^{-|m|}}{\sqrt{\pi}\,\Gamma(|m|+1/2+n)},\\[0.5ex]
\bar{p}_0&= \frac{\sqrt{\pi}\,\Gamma(1/2-n)}{\sqrt{2}},\\[0.5ex]
\bar{q}_0&= \cos(n\,\pi)\,\frac{\sqrt{2}}{\sqrt{\pi}\,\Gamma(n+1/2)}.
\end{align}

\subsection{Toroidal Electromagnetic Angular Momentum Flux}
The outward flux of toroidal angular momentum across a constant-$z$ surface is
\begin{align}
T_\phi(z) = -\oint\oint {\cal J} \,b_\phi\,b^{\,\mu}\,d\eta\,d\phi,
\end{align}
where
\begin{equation}
{\cal J} = (\nabla\mu\times\nabla\eta\cdot\nabla\phi)^{-1} = h^3\,\sinh\mu.
\end{equation}
Now,
\begin{align}
b^{\,\mu} &= {\bf b}\cdot\nabla\mu = {\rm i}\,\frac{\partial V}{\partial \mu}\,|\nabla\mu|^2 = {\rm i}\,\frac{\sinh\mu}{h^2}\,\frac{\partial V}{\partial z},\\[0.5ex]
b^{\,\phi}&= {\cal J}\,\nabla\mu\times\nabla \eta\cdot\nabla V = n\,V,
\end{align}
so
\begin{align}
T_\phi(z) &= -\frac{{\rm i}\,n\,\pi}{2}\oint \frac{z^2-1}{z-\cos\eta}\left(\frac{\partial V}{\partial z}\,V^\ast -\frac{\partial V^{\ast}}{\partial z}\,V\right)d\eta\nonumber\\[0.5ex]
&= - {\rm i}\,n\,\pi^2\sum_{m}\, (z^2-1)\left(\frac{dU_m}{dz}\,F_{m}^\ast -\frac{dU_m^\ast}{dz}\,F_{m}\right)\nonumber\\[0.5ex]
&= -{\rm i}\,n\,\pi^2\sum_{m}(p_m\,q_m^\ast-q_m\,p_m^{\ast})\,(z^2-1)\left(\frac{dP_{|m|-1/2}^{\,n}}{dz}\,Q_{|m|-1/2}^{\,n}- \frac{dQ_{|m|-1/2}^{\,n}}{dz}\,P_{|m|-1/2}^{\,n}\right)\nonumber\\[0.5ex]
& ={\rm i}\,n\,\pi^2\sum_{m}(p_m\,q_m^\ast-q_m\,p_m^{\ast})\,(z^2-1)\,{\cal W}[P_{|m|-1/2}^{\,n},Q_{|m|-1/2}^{\,n}].
\end{align}
But,
\begin{equation}
{\cal W}[P_{|m|-1/2}^{\,n},Q_{|m|-1/2}^{\,n}]= \frac{\cos(n\,\pi)}{1-z^2}\,\frac{\Gamma(|m|+1/2+n)}{\Gamma(|m|+1/2-n)},
\end{equation}
so
\begin{equation}
T_\phi(z) = 2\pi^2\,n\,\cos(n\,\pi)\sum_m\frac{\Gamma(|m|+1/2+n)}{\Gamma(|m|+1/2-n)}\,{\rm Im}(p_m\,q_m^\ast),
\end{equation}
or
\begin{equation}
T_\phi(z) = 2\pi^2\,n\,\sum_m{\rm Im}(\hat{p}_m\,\hat{q}_m^\ast)\,h_m,
\end{equation}
where
\begin{align}
h_{m\neq 0} &= \frac{2}{|m|},\\[0.5ex]
h_0 & = 1.
\end{align}

\section{Resistive  Wall Physics}
\subsection{Resistive Wall}
Let the resistive wall extend from $\mu=\mu_w$ to $\mu=\mu_w-\bar{d}_w\,\sinh\mu_w$, where $\bar{d}_w\ll 1$ is a positive constant. In other words, $\mu=\mu_w$ is the inner surface of the wall,
and $\mu=\mu_w-\bar{d}_w\,\sinh\mu_w$ is the outer surface. The physical wall thickness is
\begin{equation}
d(\eta)= \frac{\bar{d}_w\,\sinh\mu_w}{|\nabla \mu|} = g_w(\eta)\,\bar{d}_w,
\end{equation}
where
\begin{equation}
g_w(\eta) = \frac{(z_w^2-1)^{1/2}}{z_w-\cos\eta},
\end{equation}
and $z_w=\cosh\mu_w$. 
Let the electrical conductivity of the wall material vary as
\begin{equation}
\sigma(\eta) = \frac{\bar{\sigma}_w}{g_w^{\,2}(\eta)},
\end{equation}
where $\bar{\sigma}_w$ is a positive constant. It follows that $\sigma\,d^{\,2}=\bar{\sigma}_w\,\bar{d}_w^{\,2}$. 

\subsection{Wall Matching Conditions}
If we write
\begin{equation}
{\bf b} = \nabla\times{\bf A}
\end{equation}
in the vacuum region then the boundary conditions at the wall are 
\begin{align}
\left.{\bf n}_w\times {\bf A}\right|_{z_{w-}} &= \frac{1}{\cosh\lambda}\left.{\bf n}_w\times {\bf A}\right|_{z_{w+}} \\[0.5ex]
\left.{\bf n}_w\times (\nabla\times{\bf A})\right|_{z_{w+}}&= -\frac{\lambda\,\tanh\lambda}{\bar{d}_w\,g_w}\,\left.{\bf n}_w\times({\bf n}_w\times{\bf A})\right|_{z_{w+}}+
\frac{\left.{\bf n}_w\times (\nabla\times{\bf A})\right|_{z_{w-}}}{\cosh\lambda},\\[0.5ex]
\lambda &=\sqrt{\mu_0\,R_0^{\,2}\,\bar{\sigma}_w\,\bar{d}_w^{\,2}\,\gamma},
\end{align}
where $\gamma$ is the growth-rate of the magnetic perturbation. Here, ${\bf n}_w= -{\bf e}_\mu$ is an outward unit normal vector to the wall. Now,
\begin{align}
\nabla\times{\bf A} &= \frac{1}{h^2\,\sinh\mu}\left(\frac{\partial \hat{A}_\phi}{\partial \eta}-\frac{\partial\hat{A}_\eta}{\partial\phi}\right){\bf e}_\mu
+  \frac{1}{h^2\,\sinh\mu}\left(\frac{\partial \hat{A}_\mu}{\partial \phi}-\frac{\partial\hat{A}_\phi}{\partial\mu}\right){\bf e}_\eta\nonumber\\[0.5ex]
&\phantom{=}
+\frac{1}{h^2}\left(\frac{\partial \hat{A}_\eta}{\partial \mu}-\frac{\partial\hat{A}_\mu}{\partial\eta}\right){\bf e}_\phi,
\end{align}
where
\begin{align}
\hat{A}_\mu &= h\,A_\mu,\\[0.5ex]
\hat{A}_\eta&= h\,A_\eta,\\[0.5ex]
\hat{A}_\phi &= h\,\sinh\mu\,A_\phi.
\end{align}
Furthermore,
\begin{align}
{\bf n}_w\times {\bf A} &= -{\bf e}_\mu\times {\bf A} = A_\phi\,{\bf e}_\eta - A_\eta\,{\bf e}_\phi,\\[0.5ex]
{\bf n}_w\times ({\bf n}_w\times {\bf A})&= -{\bf e}_\mu\times ({\bf n}_w\times {\bf A} )= -A_\eta\,{\bf e}_\eta-A_\phi\,{\bf e}_\phi,\\[0.5ex]
{\bf n}_w\times (\nabla\times {\bf A}) &= -{\bf e}_\mu\times(\nabla\times {\bf A}) = \frac{1}{h^2}\left(\frac{\partial \hat{A}_\eta}{\partial \mu}-\frac{\partial\hat{A}_\mu}{\partial\eta}\right)\,{\bf e}_\eta- \frac{1}{h^2\,\sinh\mu}\left(\frac{\partial \hat{A}_\mu}{\partial \phi}-\frac{\partial\hat{A}_\phi}{\partial\mu}\right){\bf e}_\phi.
\end{align}
Thus, the wall matching conditions become
\begin{align}
\left.\hat{A}_\eta\right|_{z_{w-}}&= \frac{1}{\cosh\lambda}\left.\hat{A}_\eta\right|_{z_{w+}},\\[0.5ex]
\left.\hat{A}_\phi\right|_{z_{w+}}&= \frac{1}{\cosh\lambda}\,\left.\hat{A}_\phi\right|_{z_{w-}},\\[0.5ex]
\left(\frac{\partial \hat{A}_\eta}{\partial \mu}-\frac{\partial\hat{A}_\mu}{\partial\eta}\right)_{z_{w+}}
&=\frac{\lambda\,\tanh\lambda}{\bar{d}_w\,\sinh\mu_w}\left.\hat{A}_\eta\right|_{z_{w+}} + \frac{1}{\cosh\lambda}\left(\frac{\partial \hat{A}_\eta}{\partial \mu}-\frac{\partial\hat{A}_\mu}{\partial\eta}\right)_{z_{w-}},\\[0.5ex]
\left(\frac{\partial \hat{A}_\mu}{\partial \phi}-\frac{\partial\hat{A}_\phi}{\partial\mu}\right)_{z_{w+}}&= -\frac{\lambda\,\tanh\lambda}{\bar{d}_w\,\sinh\mu_w}\left.\hat{A}_\phi\right|_{\mu_{z+}}+\frac{1}{\cosh\lambda} \left(\frac{\partial \hat{A}_\mu}{\partial \phi}-\frac{\partial\hat{A}_\phi}{\partial\mu}\right)_{z_{w-}}.
\end{align}

Let
\begin{equation}
C(z,\eta,\phi) = \frac{\partial \hat{A}_\eta}{\partial \phi}- \frac{\partial \hat{A}_\phi}{\partial \eta}.
\end{equation}
The wall matching conditions reduce to 
\begin{align}
C(z_{w-},\eta,\phi) &= \frac{1}{\cosh\lambda}\,C(z_{w+},\eta,\phi),\\[0.5ex]
\frac{\partial C(z_{w+},\eta,\phi) }{\partial z}& = \frac{\lambda\,\tanh\lambda}{\bar{d}_w\,\sinh^2\mu_w}\,C(z_{w+},\eta,\phi) +\frac{1}{\cosh\lambda}\,\frac{\partial C(z_{w-},\eta,\phi) }{\partial z}.
\end{align}
However, if
\begin{equation}
{\bf b} = {\rm i}\,\nabla V =\nabla\times {\bf A}
\end{equation}
then
\begin{equation}
C = -{\rm i}\,h\,\sinh\mu\,\frac{\partial V}{\partial \mu} = -{\rm i}\,h\,(z^2-1)\,\frac{\partial V}{\partial z}.
\end{equation}
Thus,
\begin{align}
C &= -{\rm i}\,\frac{z^2-1}{z-\cos\eta}\sum_m\left[\frac{U_m}{2\,(z-\cos\eta)^{1/2}} + (z-\cos\eta)^{1/2}\,\frac{dU_m}{dz}\right]{\rm e}^{-{\rm i}\,(m\,\eta+n\,\phi)},\\[0.5ex]
\frac{\partial C}{\partial z} &= -{\rm i}\sum_m\left[\frac{(3/4)\,\sin^2\eta}{(z-\cos\eta)^{5/2}}-\frac{(1/2)\,\cos\eta}{(z-\cos\eta)^{3/2}}+ \frac{m^2+n^2/(z^2-1)}{(z-\cos\eta)^{1/2}}\right]
U_m\,{\rm e}^{-{\rm i}\,(m\,\eta+n\,\phi)}.
\end{align}
It follows that
\begin{align}
\sum_m\left[\frac{U_m}{2}+(z-\cos\eta)\,\frac{dU_m}{dz}\right]_{z_{w-}}{\rm e}^{-{\rm i}\,m\,\eta}= \frac{1}{\cosh\lambda}\sum_m\left[\frac{U_m}{2}+(z-\cos\eta)\,\frac{dU_m}{dz}\right]_{z_{w+}}{\rm e}^{-{\rm i}\,m\,\eta},\\[0.5ex]
\left.\sum_m\left[\frac{3}{4}\,\sin^2\eta-\frac{1}{2}\,(z-\cos\eta)\,\cos\eta+ (z-\cos\eta)^2\left(m^2+\frac{n^2}{z^2-1}\right)\right]
U_m\,{\rm e}^{-{\rm i}\,m\,\eta}\right|_{z_{w+}}=\nonumber\\[0.5ex]
F(\lambda) \sum_m(z-\cos\eta)\left[\frac{U_m}{2}+(z-\cos\eta)\,\frac{dU_m}{dz}\right]_{z_{w+}}{\rm e}^{-{\rm i}\,m\,\eta}\nonumber\\[0.5ex]
+\frac{1}{\cosh\lambda}\left.\sum_m\left[\frac{3}{4}\,\sin^2\eta-\frac{1}{2}\,(z-\cos\eta)\,\cos\eta+ (z-\cos\eta)^2\left(m^2+\frac{n^2}{z^2-1}\right)\right]
U_m\,{\rm e}^{-{\rm i}\,m\,\eta}\right|_{z_{w-}},
\end{align}
where
\begin{equation}
F(\lambda)= \frac{\lambda\,\tanh\lambda}{\bar{d}_w}.
\end{equation}
Thus, we can write
\begin{align}
\sum_{m'}I_{mm'}\,U_{m'}(z_{w-}) &= \frac{1}{\cosh\lambda}\sum_{m'}I_{mm'}\,U_{m'}(z_{w+}),\\[0.5ex]
\sum_{m'}J_{mm'}\,U_{m'}(z_{w+})&= F(\lambda)\sum_{m',m''}K_{mm''}\,I_{m''m'}\,U_{m'}(z_{w+}) + \frac{1}{\cosh\lambda}\sum_{m'}J_{mm'}\,U_{m'}(z_{w-}),
\end{align}
where
\begin{align}
I_{mm'}&= \left(\frac{1}{2}+z\,\frac{d}{dz}\right)\delta_{mm'}-\frac{1}{2}\,\frac{d}{dz}\,(\delta_{m\,m'+1}+\delta_{m\,m'-1}),\\[0.5ex]
J_{mm'}&= \left[\frac{5}{8} + \left(\frac{1}{2}+z^2\right)\left(m^2+\frac{n^2}{z^2-1}\right)\right]\delta_{mm'}
-z\left[\frac{1}{4}+ \left(m^2+\frac{n^2}{z^2-1}\right)\right](\delta_{m\,m'+1}+\delta_{m\,m'-1})\nonumber\\[0.5ex]
&\phantom{=}+\left[-\frac{1}{16}+\frac{1}{4} \left(m^2+\frac{n^2}{z^2-1}\right)\right](\delta_{m\,m'+2}+\delta_{m\,m'-2}),\\[0.5ex]
K_{mm'} &= z\,\delta_{mm'} - \frac{1}{2}\,(\delta_{m\,m'+1}+\delta_{m\,m'-1}).
\end{align}

\subsection{Vacuum Solution}
Now, 
\begin{equation}
U_m(z) = \bar{p}_m\,\hat{p}_{m-}\,P_{|m|-1/2}^{\,n}(z)
\end{equation}
in the region $z<z_w$, whereas 
\begin{equation}
U_m(z) = \bar{p}_m\,\hat{p}_{m+}\,P_{|m|-1/2}^{\,n}(z) + \bar{q}_m\,\hat{q}_{m+}\,Q_{|m|-1/2}^{\,n}(z) 
\end{equation}
in the region $z>z_w$. 
Let $\underline{\underline{I}}_{\,p}$ be the matrix of the
\begin{equation}
\left\{\left[\left(\frac{1}{2}+z\,\frac{d}{dz}\right)\delta_{mm'}-\frac{1}{2}\,\frac{d}{dz}\,(\delta_{m\,m'+1}+\delta_{m\,m'-1})\right]P_{|m'|-1/2}^{\,n}(z)\right\}_{z_w}\bar{p}_{m'}
\end{equation}
values.
Let $\underline{\underline{I}}_{\,q}$ be the matrix of the
\begin{equation}
\left\{\left[\left(\frac{1}{2}+z\,\frac{d}{dz}\right)\delta_{mm'}-\frac{1}{2}\,\frac{d}{dz}\,(\delta_{m\,m'+1}+\delta_{m\,m'-1})\right]Q_{|m'|-1/2}^{\,n}(z)\right\}_{z_w}\bar{q}_{m'}
\end{equation}
values. 
Let $\underline{\underline{J}}_{\,p}$ be the matrix of the 
\begin{align}
 &\left\{\left[\frac{5}{8} + \left(\frac{1}{2}+z^2\right)\left(m^2+\frac{n^2}{z^2-1}\right)\right]\delta_{mm'}
-z\left[\frac{1}{4}+ \left(m^2+\frac{n^2}{z^2-1}\right)\right](\delta_{m\,m'+1}+\delta_{m\,m'-1})\right.\nonumber\\[0.5ex]
&\phantom{=}\left.+\left[-\frac{1}{16}+\frac{1}{4} \left(m^2+\frac{n^2}{z^2-1}\right)\right](\delta_{m\,m'+2}+\delta_{m\,m'-2})\right\}P_{|m'|-1/2}^{\,n}(z_w)\,\bar{p}_{m'}
\end{align}
values. Let $\underline{\underline{J}}_{\,q}$ be the matrix of the 
\begin{align}
 &\left\{\left[\frac{5}{8} + \left(\frac{1}{2}+z^2\right)\left(m^2+\frac{n^2}{z^2-1}\right)\right]\delta_{mm'}
-z\left[\frac{1}{4}+ \left(m^2+\frac{n^2}{z^2-1}\right)\right](\delta_{m\,m'+1}+\delta_{m\,m'-1})\right.\nonumber\\[0.5ex]
&\phantom{=}\left.+\left[-\frac{1}{16}+\frac{1}{4} \left(m^2+\frac{n^2}{z^2-1}\right)\right](\delta_{m\,m'+2}+\delta_{m\,m'-2})\right\}Q_{|m'|-1/2}^{\,n}(z_w)\,\bar{q}_{m'}
\end{align}
values. 
Finally, let $\underline{\underline{K}}$ be the matrix of the 
\begin{equation}
z_w\,\delta_{mm'} -\frac{1}{2}\,(\delta_{m\,m'+1}+\delta_{m\,m'-1})
\end{equation}
values. Likewise, let $\underline{\hat{p}}_{\,+}$ be the vector of the $\hat{p}_{m+}$ values, et cetera. Thus, we
obtain
\begin{align}
\underline{\underline{I}}_{\,p}\,\underline{\hat{p}}_{\,-} &= \frac{1}{\cosh\lambda}\left(\underline{\underline{I}}_{\,p}\,\underline{\hat{p}}_{\,+} + \underline{\underline{I}}_{\,q}\,\underline{\hat{q}}_{\,+}\right),\\[0.5ex]
\underline{\underline{J}}_{\,p}\,\underline{\hat{p}}_{\,+}+ \underline{\underline{J}}_{\,q}\,\underline{\hat{q}}_{\,+} &=
F(\lambda)\,\underline{\underline{K}}\left(\underline{\underline{I}}_{\,p}\,\underline{\hat{p}}_{\,+}+ \underline{\underline{I}}_{\,q}\,\underline{\hat{q}}_{\,+} \right)
+\frac{1}{\cosh\lambda} \,\underline{\underline{J}}_{\,p}\,\underline{\hat{p}}_{\,-},
\end{align}
which can be rearranged to give 
\begin{equation}\label{e73}
\left[\tanh^2\lambda\,\underline{\underline{J}}_{\,p}-F(\lambda)\,\underline{\underline{\hat{I}}}_{\,p}\right]\underline{\hat{p}}_{\,+}+
\left[\underline{\underline{J}}_{\,pq}+\tanh^2\lambda\,\underline{\underline{J}}_{\,qp} - F(\lambda)\,\underline{\underline{\hat{I}}}_{\,q}\right]\underline{\hat{q}}_{\,+},
\end{equation}
where
\begin{align}
\underline{\underline{\hat I}}_p &= \underline{\underline{K}}\,\underline{\underline{I}}_p,\\[0.5ex]
\underline{\underline{\hat I}}_q &= \underline{\underline{K}}\,\underline{\underline{I}}_q,\\[0.5ex]
\underline{\underline{J}}_{\,pq} &=\underline{\underline{J}}_{\,q}- \underline{\underline{J}}_{\,p}\,\underline{\underline{I}}_{\,p}^{-1}\,\underline{\underline{I}}_{\,q},\\[0.5ex]
\underline{\underline{J}}_{\,qp} &= \underline{\underline{J}}_{\,p}\,\underline{\underline{I}}_{\,p}^{-1}\,\underline{\underline{I}}_{\,q}.
\end{align}

Now, $z_w\sim 1/\bar{b}_w$, where $\bar{b}_w$ is the mean wall minor radius. 
In the large aspect-ratio limit $b_w\ll 1$, we have $\underline{\underline{I}}_{\,p}\sim{\cal O}(1)$, $\underline{\underline{I}}_{\,q}\sim{\cal O}(1)$, 
$\underline{\underline{J}}_{\,p}\sim{\cal O}(1/\bar{b}_w^{\,2})$, $\underline{\underline{J}}_{\,q}\sim{\cal O}(1/\bar{b}_w^{\,2})$, 
$\underline{\underline{K}}_{\,p}\sim{\cal O}(1/\bar{b}_w)$, and $\underline{\underline{K}}_{\,q}\sim{\cal O}(1/\bar{b}_w)$. It follows that
$\underline{\underline{J}}_{\,pq} \sim{\cal O}(1/\bar{b}_w^{\,2})$ and $\underline{\underline{J}}_{\,qp} \sim{\cal O}(1/\bar{b}_w^{\,2})$. 
Thus, the ratio of the first to the second term multiplying $\underline{p}_{\,+}$ in Eq.~(\ref{e73}) is 
\begin{equation}
\tanh\lambda \,\frac{\bar{d}_w}{\lambda\,\bar{b}_w}.
\end{equation}
However, the wall analysis is premised on the assumption that
\begin{equation}
\frac{\bar{d}_w}{\lambda\,\bar{b}_w}\ll 1.
\end{equation}
Hence, the first term is negligible with respect to the second, irrespective of the value of $\lambda$. The
ratios of the three terms multiplying $\underline{q}_{\,+}$ in Eq.~(\ref{e73}) are
\begin{equation}
\frac{\bar{d}_w}{\lambda\,\bar{b}_w},~ \tanh^2\lambda\,\frac{\bar{d}_w}{\lambda\,\bar{b}_w},~ \tanh\lambda.
\end{equation}
Thus, in the thin-shell limit $\lambda\ll 1$, the second term is negligible with respect to the first. In the thick-shell limit, $\lambda\gg 1$, the third term is
dominant. Thus, we can neglect the second term. Hence, we deduce that
\begin{equation}\label{e88}
\underline{\hat{q}}_{\,+} = \underline{\underline{\cal F}}\,\underline{\hat{p}}_{\,+},
\end{equation}
where
\begin{equation}
\underline{\underline{\cal F}}= 
\left[\underline{\underline{J}}_{\,pq}- F(\lambda)\,\underline{\underline{\hat{I}}}_{\,q}\right]^{-1}F(\lambda)\,\underline{\underline{\hat{I}}}_{\,p}.
\end{equation}

\section{Plasma/Vacuum Interface}
\subsection{Matching at Plasma/Vacuum Interface}
The plasma/vacuum interface lies at $r=\epsilon$. In the vacuum region between the interface and the wall, 
\begin{equation}
V(z,\eta) =\sum_m (z-\cos\eta)^{1/2}\left[\bar{p}_{m}\,\hat{p}_{m+}\,P_{|m|-1/2}^{\,n}(z)+\bar{q}_m\,\hat{q}_{m+}\,Q_{|m|-1/2}^{\,n}(z)\right]{\rm e}^{-{\rm i}\,m\,\eta}. 
\end{equation}
Thus, if we write
\begin{align}\label{e90}
V_(r,\theta) &= \sum_m V_m(r)\,{\rm e}^{\,{\rm i}\,m\,\theta},\\[0.5ex]
\psi(r,\theta) & = \sum_m \psi_m(r)\,{\rm e}^{\,{\rm i}\,m\,\theta},\label{e91}
\end{align}
then
\begin{align}
\underline{V}&= \underline{\underline{{\cal P}}}\,\underline{\hat{p}}_{\,+}+ \underline{\underline{{\cal Q}}}\,\underline{\hat{q}}_{\,+},\\[0.5ex]
\underline{\psi}&= \underline{\underline{{\cal R}}}\,\underline{\hat{p}}_{\,+}+ \underline{\underline{{\cal S}}}\,\underline{\hat{q}}_{\,+},
\end{align}
where $\underline{V}$ is the vector of the $V_m(\epsilon)$ values, $\underline{\psi}$ is the vector of the $\psi_m$ values, $\underline{\underline{{\cal P}}}$ is the
matrix of the
\begin{equation}
{\cal P}_{mm'}=\bar{p}_{m'}\,\oint_{r=\epsilon}(z-\cos\eta)^{1/2}\,P_{|m'|-1/2}^{\,n}(z)\,\exp[-{\rm i}\,(m\,\theta+m'\,\eta)]\,\frac{d\theta}{2\pi}
\end{equation}
values, 
$\underline{\underline{{\cal Q}}}$ is the
matrix of the
\begin{equation}
{\cal Q}_{mm'}=\bar{q}_{m'}\oint_{r=\epsilon}(z-\cos\eta)^{1/2}\,Q_{|m'|-1/2}^{\,n}(z)\,\exp[-{\rm i}\,(m\,\theta+m'\,\eta)]\,\frac{d\theta}{2\pi}
\end{equation}
values, $\underline{\underline{{\cal R}}}$ is the matrix of the 
\begin{align}\label{e354}
{\cal R}_{mm'} &=\bar{p}_{m'}\oint_{r=\epsilon}
\left\{\left[\frac{1}{2}\,(z-\cos\eta)^{-1/2}\,P_{|m'|-1/2}^{\,n}(z)+(z-\cos\eta)^{1/2}\,\frac{dP_{|m'|-1/2}^{\,n}}{dz}\right]{\cal J}\,\nabla r\cdot \nabla z
\right.\nonumber\\[0.5ex]&
\left.\phantom{=}+\left[\frac{1}{2}\,(z-\cos\eta)^{-1/2}\,\sin\eta-{\rm i}\,m'\,(z-\cos\eta)^{1/2}\right]P_{|m'|-1/2}^{\,n}(z)\,{\cal J}\,\nabla r\cdot \nabla \eta
\right\}\nonumber\\[0.5ex] &
\phantom{=}\times\exp[-{\rm i}\,(m\,\theta+m'\,\eta)]\,\frac{d\theta}{2\pi}
\end{align}
values, and 
$\underline{\underline{{\cal S}}}$ is the matrix of the 
\begin{align}
{\cal S}_{mm'} &=\bar{q}_{m'}\oint_{r=\epsilon}
\left\{\left[\frac{1}{2}\,(z-\cos\eta)^{-1/2}\,Q_{|m'|-1/2}^{\,n}(z)+(z-\cos\eta)^{1/2}\,\frac{dQ_{|m'|-1/2}^{\,n}}{dz}\right]{\cal J}\,\nabla r\cdot \nabla z
\right.\nonumber\\[0.5ex]&
\left.\phantom{=}+\left[\frac{1}{2}\,(z-\cos\eta)^{-1/2}\,\sin\eta-{\rm i}\,m'\,(z-\cos\eta)^{1/2}\right]Q_{|m'|-1/2}^{\,n}(z)\,{\cal J}\,\nabla r\cdot \nabla \eta
\right\}\nonumber\\[0.5ex] &
\phantom{=}\times\exp[-{\rm i}\,(m\,\theta+m'\,\eta)]\,\frac{d\theta}{2\pi}
\end{align}

Equations~(\ref{e88}), (\ref{e90}), and (\ref{e91}) imply that
\begin{equation}
\underline{V}= \underline{\underline{H}}\,\underline{\psi},
\end{equation}
where
\begin{equation}
\underline{\underline{H}}\,(\underline{\underline{\cal R}}+\underline{\underline{\cal S}}\,\underline{\underline{\cal F}}) = \underline{\underline{\cal P}}+\underline{\underline{\cal Q}}\,\underline{\underline{\cal F}}.
\end{equation}

\end{document}